Fix And8.lean

Clean/Gadgets/And/And8.lean
@@ -21,7 +21,7 @@ def Assumptions (input : Inputs (F p)) :=
   let ⟨x, y⟩ := input
   x.val < 256 ∧ y.val < 256
 
-def Spec (input : Inputs (F p)) (z : F p) :=
+def Spec {sentences : PropertySet (F p)} (_ : CheckedYields sentences) (input : Inputs (F p)) (z : F p) :=
   let ⟨x, y⟩ := input
   z.val = x.val &&& y.val
 
@@ -80,7 +80,7 @@ instance elaborated : ElaboratedCircuit (F p) Inputs field where
   localLength _ := 1
   output _ i := var ⟨i⟩
 
-theorem soundness : Soundness (F p) elaborated Assumptions Spec := by
+theorem soundness sentences checked  : Soundness (F p) sentences checked elaborated Assumptions Spec := by
   intro i env ⟨ x_var, y_var ⟩ ⟨ x, y ⟩ h_input h_assumptions h_xor
   simp_all only [circuit_norm, main, Assumptions, Spec, ByteXorTable, Inputs.mk.injEq]
   have ⟨ hx_byte, hy_byte ⟩ := h_assumptions
